src/impl/TLS13.Impl.Server.fsti
@@ -1940,7 +1940,7 @@ fn process_network_bytes
                   network_out_bytes
                   app_out_bytes /\
                 (buffer_resp.ST.response.ST.status == ST.StepOk ==>
-                  exists ch raw_received.
+                  (exists ch raw_received.
                     st1 ==
                       CM.received_client_hello_state
                         'st0
@@ -1951,6 +1951,18 @@ fn process_network_bytes
                       (Seq.slice
                         (Ghost.reveal 'raw_bytes)
                         0
-                        (SZ.v buffer_resp.ST.consumed_len))) /\
+                        (SZ.v buffer_resp.ST.consumed_len))) \/
+                  (exists fin raw_received.
+                    st1 ==
+                      CM.received_client_finished_state
+                        'st0
+                        fin
+                        raw_received /\
+                    Seq.equal
+                      raw_received
+                      (Seq.slice
+                        (Ghost.reveal 'raw_bytes)
+                        0
+                        (SZ.v buffer_resp.ST.consumed_len)))) /\
                 (buffer_resp.ST.response.ST.status == ST.NeedMoreInput ==>
                   buffer_resp.ST.consumed_len == 0sz))
